Validator.lean
@@ -2,7 +2,9 @@ import Validator.Std
 
 import Validator.Derive
 import Validator.Expr
+import Validator.Hedge
 import Validator.Learning
 import Validator.Memoize
 import Validator.Parser
+import Validator.Regex
 import Validator.Validator
