Validator/Expr.lean
@@ -1,8 +1,3 @@
-import Validator.Expr.Compress
-import Validator.Expr.Grammar
-import Validator.Expr.IfExpr
-import Validator.Expr.Language
+import Validator.Hedge.IfExpr
 import Validator.Expr.Pred
-import Validator.Expr.Regex
-import Validator.Expr.Symbol
 import Validator.Expr.TokenPred
