Validator/Hedge/Language.lean
@@ -1,0 +1,64 @@
+import Validator.Std.Hedge
+import Validator.Regex.Language
+
+namespace Hedge.Language
+
+open List (
+  append_assoc
+  append_eq_nil_iff
+  append_nil
+  cons
+  cons_append
+  cons.injEq
+  foldl_nil
+  nil
+  nil_append
+  nil_eq
+  singleton_append
+)
+
+-- Definitions
+
+def Lang (α: Type): Type := Regex.Language.Langs (Hedge.Node α)
+
+def tree {α: Type} (φ: α -> Bool) (R: Lang α): Lang α :=
+  fun xs => ∃ label children, xs = [Hedge.Node.mk label children] /\ φ label /\ R children
+
+example: Lang Nat := (tree (fun x => x = 1) (Regex.Language.or (tree (fun x => x = 1) Regex.Language.emptystr) Regex.Language.emptyset))
+
+theorem null_iff_tree {α: Type} {p: α -> Bool} {children: Lang α}:
+  Regex.Language.null (tree p children) <-> False :=
+  Iff.intro nofun nofun
+
+theorem null_tree {α: Type} {p: α -> Bool} {children: Lang α}:
+  Regex.Language.null (tree p children) = False := by
+  rw [null_iff_tree]
+
+theorem derive_iff_tree {α: Type} {p: α -> Bool} {childlang: Lang α} {label: α} {children: Hedge α} {xs: Hedge α}:
+  (Regex.Language.derive (tree p childlang) (Hedge.Node.mk label children)) xs <->
+  (Regex.Language.onlyif (p label /\ childlang children) Regex.Language.emptystr) xs := by
+  simp only [Regex.Language.derive, Regex.Language.derives, singleton_append]
+  simp only [Regex.Language.onlyif, Regex.Language.emptystr]
+  refine Iff.intro ?toFun ?invFun
+  case toFun =>
+    unfold tree
+    simp only [cons.injEq, Hedge.Node.mk.injEq]
+    intro ⟨ label', children', ⟨ ⟨ hlabel', hchildren' ⟩, hxs ⟩ , hif ⟩
+    subst_vars
+    simp only [and_true]
+    exact hif
+  case invFun =>
+    intro ⟨ hif , hxs  ⟩
+    unfold tree
+    exists label
+    exists children
+    rw [hxs]
+    simp only [true_and]
+    exact hif
+
+-- Hedge.Language.derive (Hedge.Language.tree p.eval (Denote.denote children)) a
+theorem derive_tree {α: Type} {p: α -> Bool} {childlang: Lang α} {label: α} {children: Hedge α}:
+  (Regex.Language.derive (tree p childlang) (Hedge.Node.mk label children)) =
+  (Regex.Language.onlyif (p label /\ childlang children) Regex.Language.emptystr) := by
+  funext
+  rw [derive_iff_tree]
