Validator/Learning/ImperativeCompress.lean
@@ -9,10 +9,10 @@ import Validator.Std.Vec
 
 import Validator.Parser.TokenTree
 
-import Validator.Expr.Compress
-import Validator.Expr.Grammar
-import Validator.Expr.IfExpr
-import Validator.Expr.Regex
+import Validator.Hedge.Compress
+import Validator.Hedge.Grammar
+import Validator.Hedge.IfExpr
+import Validator.Regex.Regex
 
 import Validator.Learning.ImperativeLeave
 import Validator.Learning.ImperativeEnter
