Validator/Regex.lean
@@ -1,0 +1,3 @@
+import Validator.Regex.Language
+import Validator.Regex.Regex
+import Validator.Regex.Symbol
